ovn/src/ovn_group.rs
@@ -1,0 +1,350 @@
+#![no_std]
+#![feature(register_tool)]
+#![register_tool(hax)]
+
+#[hax_lib_macros::exclude]
+extern crate hax_lib_macros;
+#[hax_lib_macros::exclude]
+use hax_lib_macros::*;
+
+#[exclude]
+use hacspec_concordium::*;
+#[exclude]
+use hacspec_concordium_derive::*;
+
+use hacspec_bls12_381::*;
+
+pub trait Z_Field : core::marker::Copy {
+    type field_type: PartialEq + Eq + Clone + Copy + hacspec_concordium::Serialize;
+
+    const q : usize;
+
+    fn random_field_elem(random : u32) -> Self::field_type;
+
+    fn field_zero() -> Self::field_type;
+    fn field_one() -> Self::field_type;
+
+    fn add(x: Self::field_type, y: Self::field_type) -> Self::field_type;
+    fn mul(x: Self::field_type, y: Self::field_type) -> Self::field_type;
+}
+
+/** Interface for group implementation */
+pub trait Group<Z: Z_Field> : core::marker::Copy {
+    type group_type: PartialEq + Eq + Clone + Copy + hacspec_concordium::Serialize;
+
+    const g: Self::group_type; // Generator (elemnent of group)
+
+    fn random_group_elem(random : u32) -> Self::group_type;
+
+    fn g_pow(x: Z::field_type) -> Self::group_type;
+    fn pow(g: Self::group_type, x: Z::field_type) -> Self::group_type; // TODO: Link with q
+    fn group_one() -> Self::group_type;
+    fn prod(x: Self::group_type, y: Self::group_type) -> Self::group_type;
+    fn inv(x: Self::group_type) -> Self::group_type;
+    fn div(x: Self::group_type, y: Self::group_type) -> Self::group_type;
+}
+
+// struct eligible_votes {
+//     v_id : u32,
+// }
+
+// /** number of parties */
+// const n : u32 = 3u32;
+// const P : [eligible_votes; 3] = // n = 3
+//     [eligible_votes {v_id: 0},
+//      eligible_votes {v_id: 1},
+//      eligible_votes {v_id: 2}];
+
+// use concordium_contracts_common::*;
+// extern crate concordium_std;
+
+// use hacspec_sha256::*;
+
+/** TODO: Hash function */
+pub fn Hash<Z : Z_Field, G : Group<Z>>(v : (G::group_type, G::group_type, G::group_type)) -> Z::field_type {
+    let (a, b, c) = v;
+    Z::field_one()
+}
+
+#[derive(Serialize, SchemaType, Clone, Copy)]
+struct SchnorrZKPCommit<Z : Z_Field, G: Group<Z>> {
+    u: G::group_type,
+    c: Z::field_type,
+    z: Z::field_type,
+}
+
+/** Non-interactive Schnorr proof using Fiat-Shamir heuristics */
+// https://crypto.stanford.edu/cs355/19sp/lec5.pdf
+pub fn schnorr_ZKP<Z : Z_Field, G: Group<Z>>(random: u32, g_pow_x: G::group_type, x: Z::field_type) -> SchnorrZKPCommit<Z, G> {
+    let r = Z::random_field_elem(random);
+    let u = G::g_pow(r);
+    let c = Hash::<Z,G>((G::g, g_pow_x, u));
+    let z = Z::add(r , Z::mul(c , x) );
+
+    return SchnorrZKPCommit { u, c, z };
+}
+
+// https://crypto.stanford.edu/cs355/19sp/lec5.pdf
+pub fn schnorr_ZKP_validate<Z : Z_Field, G: Group<Z>>(g_pow_x: G::group_type, pi: SchnorrZKPCommit<Z, G>) -> bool {
+    pi.c == Hash::<Z,G>((G::g, g_pow_x, pi.u)) && G::g_pow(pi.z) == G::prod(pi.u , G::pow(g_pow_x, pi.c))
+}
+
+#[hax::contract_state(contract = "OVN")]
+// #[cfg_attr(not(feature = "hax_compilation"), contract_state(contract = "OVN"))]
+#[derive(Serialize, SchemaType, Clone, Copy)]
+pub struct OvnContractState<Z : Z_Field, G: Group<Z>, const n: usize> {
+    zkp_random: u32,
+
+    g_pow_xis: [G::group_type; n],
+    zkp_xis: [SchnorrZKPCommit<Z, G>; n],
+
+    commit_vis: [u32; n],
+
+    g_pow_xi_yi_vis: [G::group_type; n],
+    zkp_vis: [u32; n],
+
+    tally: u32,
+}
+
+#[hax::init(contract = "OVN")]
+// #[cfg_attr(not(feature = "hax_compilation"), init(contract = "OVN"))]
+pub fn init_ovn_contract<Z : Z_Field, G: Group<Z>, const n: usize>(
+    _: &impl HasInitContext,
+) -> InitResult<OvnContractState<Z,G,n>> {
+    Ok(OvnContractState::<Z,G,n> {
+        zkp_random: 0, // TODO
+
+        g_pow_xis: [G::group_one(); n],
+        zkp_xis: [SchnorrZKPCommit::<Z, G> { u: G::group_one(), z: Z::field_zero(), c: Z::field_zero() }; n],
+
+        commit_vis: [0; n],
+
+        g_pow_xi_yi_vis: [G::group_one(); n],
+        zkp_vis: [0; n],
+
+        tally: 0,
+    })
+}
+
+/** Currently randomness needs to be injected */
+pub fn select_private_voting_key<Z : Z_Field, G : Group<Z>>(random: u32) -> G::group_type {
+    G::random_group_elem(random) // x_i \in_R Z_q;
+}
+
+#[derive(Serialize, SchemaType)]
+pub struct RegisterParam<Z : Z_Field> {
+    rp_i: u32,
+    rp_xi: Z::field_type,
+}
+
+/** Primary function in round 1 */
+#[hax::receive(contract = "OVN", name = "register", parameter = "RegisterParam")]
+// #[cfg_attr(not(feature = "hax_compilation"), receive(contract = "OVN", name = "register", parameter = "RegisterParam"))]
+pub fn register_vote<Z : Z_Field, G : Group<Z>, const n : usize, A: HasActions>(
+    ctx: &impl HasReceiveContext,
+    state: OvnContractState<Z, G, n>,
+) -> Result<(A, OvnContractState<Z, G, n>), ParseError> {
+    let params: RegisterParam<Z> = ctx.parameter_cursor().get()?;
+    let g_pow_xi = G::g_pow(params.rp_xi);
+
+    let zkp_xi = schnorr_ZKP::<Z, G>(state.zkp_random, g_pow_xi, params.rp_xi);
+
+    let mut register_vote_state_ret = state.clone();
+    register_vote_state_ret.g_pow_xis[params.rp_i as usize] = g_pow_xi;
+    register_vote_state_ret.zkp_xis[params.rp_i as usize] = zkp_xi;
+
+    Ok((A::accept(), register_vote_state_ret))
+}
+
+#[derive(Serialize, SchemaType)]
+pub struct CastVoteParam<Z : Z_Field> {
+    cvp_i: u32,
+    cvp_xi: Z::field_type,
+    cvp_vote: bool,
+}
+
+pub fn compute_group_element_for_vote<Z : Z_Field, G: Group<Z>, const n: usize>(
+    i: u32,
+    xi: Z::field_type,
+    vote: bool,
+    xis: [G::group_type; n],
+) -> G::group_type {
+    let mut prod1 = G::group_one();
+    for j in 0..(i - 1) as usize {
+        prod1 = G::prod(prod1, xis[j]);
+    }
+    let mut prod2 = G::group_one();
+    for j in (i + 1) as usize..n {
+        prod2 = G::prod(prod2, xis[j]);
+    }
+    let Yi = G::div(prod1, prod2);
+    // implicityly: Y_i = g^y_i
+    G::prod(G::pow(Yi, xi), G::g_pow(if vote { Z::field_one() } else { Z::field_zero() }))
+}
+
+pub fn commit_to<Z : Z_Field, G: Group<Z>>(x: G::group_type) -> u32 {
+    0
+}
+
+/** Commitment before round 2 */
+#[hax::receive(contract = "OVN", name = "commit_to_vote", parameter = "CastVoteParam")]
+// #[cfg_attr(not(feature = "hax_compilation"), receive(contract = "OVN", name = "commit_to_vote", parameter = "CastVoteParam"))]
+pub fn commit_to_vote<Z : Z_Field, G : Group<Z>, const n : usize, A: HasActions>(
+    ctx: &impl HasReceiveContext,
+    state: OvnContractState<Z, G, n>,
+) -> Result<(A, OvnContractState<Z, G, n>), ParseError> {
+    let params: CastVoteParam<Z> = ctx.parameter_cursor().get()?;
+
+    for i in 0..n {
+        if !schnorr_ZKP_validate(state.g_pow_xis[i], state.zkp_xis[i]) {
+            return Err(ParseError {});
+        }
+    }
+
+    let g_pow_xi_yi_vi = compute_group_element_for_vote::<Z, G, n>(params.cvp_i, params.cvp_xi, params.cvp_vote, state.g_pow_xis);
+    let commit_vi = commit_to::<Z, G>(g_pow_xi_yi_vi);
+
+    let mut commit_to_vote_state_ret = state.clone();
+    commit_to_vote_state_ret.commit_vis[params.cvp_i as usize] = commit_vi;
+    Ok((A::accept(), commit_to_vote_state_ret))
+}
+
+/** Cramer, Damgård and Schoenmakers (CDS) technique */
+pub fn ZKP_one_out_of_two<Z : Z_Field, G: Group<Z>>(g_pow_vi: G::group_type, vi: bool) -> u32 {
+    32 // TODO
+}
+
+/** Primary function in round 2, also opens commitment */
+#[hax::receive(contract = "OVN", name = "cast_vote", parameter = "CastVoteParam")]
+// #[cfg_attr(not(feature = "hax_compilation"), receive(contract = "OVN", name = "cast_vote", parameter = "CastVoteParam"))]
+pub fn cast_vote<Z : Z_Field, G : Group<Z>, const n : usize, A: HasActions>(
+    ctx: &impl HasReceiveContext,
+    state: OvnContractState<Z, G, n>,
+) -> Result<(A, OvnContractState<Z, G, n>), ParseError> {
+    let params: CastVoteParam<Z> = ctx.parameter_cursor().get()?;
+
+    let g_pow_xi_yi_vi = compute_group_element_for_vote::<Z, G, n>(params.cvp_i, params.cvp_xi, params.cvp_vote, state.g_pow_xis);
+    let zkp_vi = ZKP_one_out_of_two::<Z, G>(g_pow_xi_yi_vi, params.cvp_vote);
+
+    let mut cast_vote_state_ret = state.clone();
+    cast_vote_state_ret.g_pow_xi_yi_vis[params.cvp_i as usize] = g_pow_xi_yi_vi;
+    cast_vote_state_ret.zkp_vis[params.cvp_i as usize] = zkp_vi;
+
+    Ok((A::accept(), cast_vote_state_ret))
+}
+
+pub fn check_valid2<Z : Z_Field, G: Group<Z>>(g_pow_xi_yi_vi: G::group_type, zkp: u32) -> bool {
+    true
+}
+
+pub fn check_commitment<Z : Z_Field, G: Group<Z>>(g_pow_xi_yi_vi: G::group_type, zkp: u32) -> bool {
+    true
+}
+
+pub struct TallyParameter {}
+#[hax::receive(contract = "OVN", name = "tally", parameter = "TallyParameter")]
+// #[cfg_attr(not(feature = "hax_compilation"), receive(contract = "OVN", name = "tally", parameter = "TallyParameter"))]
+/** Anyone can tally the votes */
+pub fn tally_votes<Z : Z_Field, G: Group<Z>, const n : usize, A: HasActions>(
+    _: &impl HasReceiveContext,
+    state: OvnContractState<Z, G, n>,
+) -> Result<(A, OvnContractState<Z, G, n>), ParseError> {
+    for i in 0..n {
+        check_valid2::<Z, G>(state.g_pow_xi_yi_vis[i], state.zkp_vis[i]);
+        check_commitment::<Z, G>(state.g_pow_xi_yi_vis[i], state.commit_vis[i]);
+        ()
+    }
+
+    let mut vote_result = G::group_one();
+    for g_pow_vote in state.g_pow_xi_yi_vis {
+        vote_result = G::prod(vote_result, g_pow_vote);
+    }
+
+    let mut tally = 0;
+    let mut curr = Z::field_zero();
+    for i in 0..n as u32 {
+        // Should be while, but is bounded by n anyways!
+        if G::g_pow(curr) == vote_result {
+            tally = i;
+        }
+
+        curr = Z::add(curr, Z::field_one());
+    }
+
+    let mut tally_votes_state_ret = state.clone();
+    tally_votes_state_ret.tally = tally;
+
+    Ok((A::accept(), tally_votes_state_ret))
+}
+
+#[cfg(test)]
+#[concordium_test]
+pub fn test_correctness<Z : Z_Field, G: Group<Z>>() {
+    let randomness: Vec<u32> = Vec::new();
+    let votes: Vec<bool> = Vec::new();
+
+    // Setup the context
+    let mut ctx = InitContextTest::empty();
+    // ctx.set_sender(ADDRESS_0);
+
+    let mut state = init_ovn_contract();
+
+    let xis = Vec::new();
+    for i in 0..n {
+        xis.push(select_private_voting_key::<Z, G>(randomness[i]));
+    }
+
+    for i in 0..n {
+        let parameter = RegisterParam {
+            rp_i: i,
+            rp_xi: xis[i],
+        };
+        let parameter_bytes = to_bytes(&parameter);
+        ctx.set_parameter(&parameter_bytes);
+
+        register_vote(ctx, state);
+    }
+
+    for i in 0..n {
+        let parameter = CastVoteParam::<Z> {
+            cvp_i: i,
+            cvp_xi: xis[i],
+            cvp_vote: votes[i],
+        };
+        let parameter_bytes = to_bytes(&parameter);
+        ctx.set_parameter(&parameter_bytes);
+
+        commit_to_vote(ctx, state);
+    }
+
+    for i in 0..n {
+        let parameter = CastVoteParam::<Z> {
+            cvp_i: i,
+            cvp_xi: xis[i],
+            cvp_vote: votes[i],
+        };
+        let parameter_bytes = to_bytes(&parameter);
+        ctx.set_parameter(&parameter_bytes);
+
+        cast_vote(ctx, state);
+    }
+
+    let parameter = TallyParameter {};
+    let parameter_bytes = to_bytes(&parameter);
+    ctx.set_parameter(&parameter_bytes);
+
+    tally_votes(ctx, state);
+
+    let mut count = 0;
+    for v in votes {
+        if v {
+            count = count + 1; // += 1 does not work correctly
+        }
+    }
+
+    claim_eq!(
+        state.tally,
+        count,
+        "The tally should equal the number of positive votes"
+    );
+}
